# generic
@prefix dc: <http://purl.org/dc/elements/1.1/> .
@prefix owl: <http://www.w3.org/2002/07/owl#> .
@prefix rdf: <http://www.w3.org/1999/02/22-rdf-syntax-ns#> .
@prefix xsd: <http://www.w3.org/2001/XMLSchema#> .
@prefix rdfs: <http://www.w3.org/2000/01/rdf-schema#> .
@prefix w3c-format: <http://www.w3.org/ns/formats/> .
@prefix foaf: <http://xmlns.com/foaf/0.1/> .
@prefix xml: <http://www.w3.org/XML/1998/namespace> .
# privacy
@prefix svpr:  <http://www.specialprivacy.eu/vocabs/processing#> .
@prefix svpu:  <http://www.specialprivacy.eu/vocabs/purposes#> .
@prefix svd:   <http://www.specialprivacy.eu/vocabs/data#> .
@prefix svdu:  <http://www.specialprivacy.eu/vocabs/duration#> .
@prefix svl:   <http://www.specialprivacy.eu/vocabs/locations#> .
@prefix svr:   <http://www.specialprivacy.eu/vocabs/recipients#> .
@prefix spl:   <http://www.specialprivacy.eu/langs/usage-policy#> .
# shacl
@prefix sh: <http://www.w3.org/ns/shacl#> .

# semcon-specific
@prefix : <http://w3id.org/semcon/ns/ontology#> .
@prefix scr: <http://w3id.org/semcon/ns/sc-resource/> .
# zamg-specific
@prefix zamg: <http://w3id.org/semcon/ns/zamg#> .
@prefix wgs: <http://www.w3.org/2003/01/geo/wgs84_pos#> .

#################################################################
#    NAMED GRAPH ==> :BaseConfiguration
#################################################################
:BaseConfiguration {

	:ContainerConfigurationInstance rdf:type :ContainerConfiguration ;
		# generic - dublin core
		dc:title "ZAMG Container" ;
		dc:description """
				This container contains information about step count
			""" ;
		dc:creator [
			rdf:type foaf:Person ;
			foaf:name "Christoph Fabianek" ;
			foaf:mbox <mailto:christoph.fabianek@gmail.com> ;
		] ;
		:hasDataConfiguration :DataConfigurationInstance .
		# :hasDataLayer scr:LayerSemantic ;		# NON-EDITABLE - assigned

	:DataConfigurationInstance rdf:type :DataConfiguration ;	
		# :isDataModelExist true ;				# NON-EDITABLE - assigned
		# :isDataConstraintExist true ;			# NON-EDITABLE - assigned
		# :isDataMappingExist false ;			# NON-EDITABLE - assigned
		# :isUsagePolicyExist true ;			# NON-EDITABLE - assigned
		# data - classifications
		:hasTag "ZAMG", "Earthquake" ;
		# data format - inspired from void
		:hasNativeSyntax w3c-format:Turtle ;
		# example data in plain string
		:hasExampleData """
		    @prefix wgs: <http://www.w3.org/2003/01/geo/wgs84_pos#> .
            @prefix zamg: <http://w3id.org/semcon/ns/zamg#> .
            @prefix scr: <http://w3id.org/semcon/ns/sc-resource/> .
            @prefix xsd: <http://www.w3.org/2001/XMLSchema#> .

            scr:data1 a zamg:DataPoint ;
            zamg:lastUpdate "2019-01-08T13:11:47.823Z"^^xsd:dateTimeStamp ;
            zamg:time "2019-01-08T12:39:31.040Z"^^xsd:dateTimeStamp ;
            zamg:magnitude 5.5 ;
            zamg:magnitudeType "M" ;
            zamg:sourceId "1816909" ;
            zamg:eventType "EARTHQUAKE" ;
            zamg:auth "QED" ;
            wgs:location [
                a wgs:Point ;
                wgs:long 131.0371 ;
                wgs:lat 30.5926 ;
                wgs:alt -35 ;
            ] ;
            .
		"""	.
}

#################################################################
#    NAMED GRAPH ==> :UsagePolicy
#################################################################
:UsagePolicy {
	:ContainerPolicy rdf:type owl:Class ; # this line should not be changed!
		owl:equivalentClass [ 
			owl:intersectionOf ( 
				[ 
					rdf:type owl:Restriction ;
					owl:onProperty spl:hasData ;
					owl:someValuesFrom svd:AnyData
				]
				[ 
					rdf:type owl:Restriction ;
					owl:onProperty spl:hasProcessing ;
					owl:someValuesFrom spl:AnyProcessing
				]
				[ 
					rdf:type owl:Restriction ;
					owl:onProperty spl:hasPurpose ;
					owl:someValuesFrom spl:AnyPurpose
				]
				[ 
					rdf:type owl:Restriction ;
					owl:onProperty spl:hasRecipient ;
					owl:someValuesFrom spl:AnyRecipient
				]
				[ 
					rdf:type owl:Restriction ;
					owl:onProperty spl:hasStorage ;
					owl:someValuesFrom spl:AnyStorage
				]
			) ;
			rdf:type owl:Class
		] .
}
	
#################################################################
#    NAMED GRAPH ==> :DataModel
#################################################################
:DataModel {
	# I have a single class, called DataPoint
	zamg:DataPoint a owl:Class ;
        rdfs:comment """
            ZAMG data is currently represented in a single class called zamg:DataPoint
        """ .

	zamg:lastUpdate a owl:DatatypeProperty, owl:FunctionalProperty ;
		rdfs:domain zamg:DataPoint ;
		rdfs:range xsd:dateTimeStamp ;
		rdfs:comment """
	        each DataPoint has a maximum of one zamg:lastUpdate property of type xsd:dateTimeStamp
		    representing when was the DataPoint (last) published
		""" .

	zamg:time a owl:DatatypeProperty, owl:FunctionalProperty ;
		rdfs:domain zamg:DataPoint ;
		rdfs:range xsd:integer ;
        rdfs:comment """
            each DataPoint has a maximum of one zamg:time property of type xsd:dateTimeStamp
            representing when was the event happened
        """ .

	zamg:magnitude a owl:DatatypeProperty, owl:FunctionalProperty ;
		rdfs:domain zamg:DataPoint ;
		rdfs:range xsd:decimal ;
        rdfs:comment """
            each DataPoint has a maximum of one zamg:magnitude property of type xsd:decimal
            representing the magnitude of the event happened
        """ .

	zamg:magnitudeType a owl:DatatypeProperty, owl:FunctionalProperty ;
		rdfs:domain zamg:DataPoint ;
		rdfs:range xsd:string ;
        rdfs:comment """
            each DataPoint has a maximum of one zamg:magnitudeType property of type xsd:string
            representing the type of magnitude from the event happened
        """ .

	zamg:sourceId a owl:DatatypeProperty, owl:FunctionalProperty ;
		rdfs:domain zamg:DataPoint ;
		rdfs:range xsd:string ;
        rdfs:comment """
            each DataPoint has a maximum of one zamg:dataSourceId property of type xsd:string
            representing the unique id of the zamg:DataPoint generated by the data source.
        """ .

	zamg:eventType a owl:DatatypeProperty, owl:FunctionalProperty ;
		rdfs:domain zamg:DataPoint ;
		rdfs:range xsd:string ;
        rdfs:comment """
            each DataPoint has a maximum of one zamg:eventType property of type xsd:string
            representing the type of the event happened (e.g., EARTHQUAKE)
        """ .

	zamg:auth a owl:DatatypeProperty, owl:FunctionalProperty ;
		rdfs:domain zamg:DataPoint ;
		rdfs:range xsd:string ;
        rdfs:comment """
            each DataPoint has a maximum of one zamg:dataSourceId property of type xsd:string
            representing the publisher of the data (e.g., expert, machine)
        """ .

	wgs:location a owl:ObjectProperty, owl:FunctionalProperty ;
		rdfs:domain zamg:DataPoint ;
		rdfs:range wgs:Point ;
        rdfs:comment """
            each DataPoint has a maximum of one wgs:location property of type wgs:Point
            representing where was the earthquake event happened
        """ .
}

#################################################################
#    NAMED GRAPH ==> :DataConstraint
#################################################################
:DataConstraint {
	scr:DataPointShape a sh:NodeShape ;
		sh:name "ZAMG data constraints" ;
		sh:targetClass zamg:DataPoint ;
		sh:description "Example data constraints for zamg:DataPoint" ;
		sh:closed true ;
		sh:property [
			sh:path rdf:type ;
			sh:maxCount 1 ;
			sh:minCount 1 ;
		] ;
		sh:property [
			sh:path zamg:lastUpdate ;
			sh:dataType xsd:dateTimeStamp ;
			sh:maxCount 1 ;
			sh:minCount 1 ;
		] ;
		sh:property [
			sh:path zamg:time ;
			sh:dataType xsd:dateTimeStamp ;
			sh:maxCount 1 ;
			sh:minCount 1 ;
		] ;
		sh:property [
			sh:path zamg:magnitude ;
			sh:maxCount 1 ;
			sh:minCount 1 ;
		] ;
		sh:property [
			sh:path zamg:magnitudeType ;
			sh:dataType xsd:string ;
			sh:maxCount 1 ;
			sh:minCount 1 ;
		] ;
		sh:property [
			sh:path zamg:sourceId ;
			sh:dataType xsd:string ;
			sh:maxCount 1 ;
			sh:minCount 1 ;
		] ;
		sh:property [
			sh:path zamg:eventType ;
			sh:dataType xsd:string ;
			sh:maxCount 1 ;
			sh:minCount 1 ;
		] ;
		sh:property [
			sh:path zamg:auth ;
			sh:dataType xsd:string ;
			sh:maxCount 1 ;
			sh:minCount 1 ;
		] ;
		sh:property [
			sh:path wgs:location ;
			sh:dataType wgs:Point ;
			sh:maxCount 1 ;
			sh:minCount 1 ;
		] ;
	.
	scr:WGSPointShape a sh:NodeShape ;
		sh:name "WGS Point data constraints" ;
		sh:targetClass wgs:Point ;
		sh:description "Data constraints for wgs:Point" ;
		sh:closed true ;
		sh:property [
			sh:path rdf:type ;
			sh:maxCount 1 ;
			sh:minCount 1 ;
		] ;
		sh:property [
			sh:path wgs:long ;
			sh:dataType xsd:decimal ;
			sh:maxCount 1 ;
			sh:minCount 1 ;
		] ;
		sh:property [
			sh:path wgs:lat ;
			sh:dataType xsd:decimal ;
			sh:maxCount 1 ;
			sh:minCount 1 ;
		] ;
		sh:property [
			sh:path wgs:alt ;
			sh:dataType xsd:decimal ;
			sh:maxCount 1 ;
			sh:minCount 1 ;
		] ;
	.
}

#################################################################
#    NAMED GRAPH ==> :DataMappings (Future)
#################################################################
:DataMapping {

}

#################################################################
#    NAMED GRAPH ==> :UserFunctions - Hydra function definitions (Future)
#################################################################
:UserFunction {

}
